map & law & bind

LambdaCDollar.v
@@ -9,52 +9,164 @@ Require Export Common.
 
 (* Terms *)
 
-Inductive tm : Type → Type := 
-| tm_val    : ∀ {V}, val V → tm V
-| tm_nonval : ∀ {V}, non V → tm V
-with val : Type → Type := 
-| val_var   : ∀ {V}, V → val V
-| val_lam   : ∀ {V}, tm ^V → val V
-| val_S₀    : ∀ {V}, val V
-with non : Type → Type :=
-| non_app   : ∀ {V}, tm V → tm V → non V
-| non_let   : ∀ {V}, tm V → tm ^V → non V
-| non_reset : ∀ {V}, tm V → tm V → non V
+Inductive tm {V} := 
+| tm_val    : val → tm
+| tm_non    : non → tm
+with val {V} := 
+| val_var   : V → val
+| val_lam   : @tm ^V → val
+| val_S₀    : val
+with non {V} :=
+| non_app   : tm → tm → non
+| non_let   : tm → @tm ^V → non
+| non_reset : tm → tm → non
 .
+Arguments tm  V : clear implicits.
+Arguments val V : clear implicits.
+Arguments non V : clear implicits.
 
-Declare Custom Entry λc_dollar_scope.
-Notation "<{ M }>" := M (at level 1, M custom λc_dollar_scope at level 99).
-Notation "( x )" := x (in custom λc_dollar_scope, x at level 99).
-Notation "{ x }" := x (in custom λc_dollar_scope at level 0, x constr).
-Notation "x" := x (in custom λc_dollar_scope at level 0, x constr at level 0).
-(* Notation tm_var_n n := (tm_var (var_n n)). *)
-(* Notation "0" := (tm_var_n 0) (in custom λc_dollar_scope at level 0). *)
-(* Notation "1" := (tm_var_n 1) (in custom λc_dollar_scope at level 0). *)
-(* Notation "2" := (tm_var_n 2) (in custom λc_dollar_scope at level 0). *)
-(* Notation "3" := (tm_var_n 3) (in custom λc_dollar_scope at level 0). *)
-(* Notation "4" := (tm_var_n 4) (in custom λc_dollar_scope at level 0). *)
-Notation "'var' v" := (tm_val (val_var v)) (in custom λc_dollar_scope at level 1, left associativity).
-Notation "0" := <{ var None }> (in custom λc_dollar_scope at level 0).
-Notation "1" := <{ var {Some None} }> (in custom λc_dollar_scope at level 0).
-Notation "2" := <{ var {Some (Some None)} }> (in custom λc_dollar_scope at level 0).
-Notation "M N" := (tm_nonval (non_app M N)) (in custom λc_dollar_scope at level 1, left associativity).
-Notation "'λ' M" := (tm_val (val_lam M))
-  (in custom λc_dollar_scope at level 90,
-   M custom λc_dollar_scope at level 99,
-   right associativity).
-Notation "M '$' N" := (tm_nonval (non_reset M N)) (in custom λc_dollar_scope at level 80, right associativity).
-(* Notation "'S₀'" := (tm_val (val_S₀)) (in custom λc_dollar_scope at level 0). *)
-Notation "'S₀' M" := <{ {tm_val (val_S₀)} (λ M) }>
-  (in custom λc_dollar_scope at level 90,
-   M custom λc_dollar_scope at level 99,
-   right associativity).
-Notation "'let' M 'in' N" := (tm_nonval (non_let M N))
-  (in custom λc_dollar_scope at level 95,
-   M custom λc_dollar_scope at level 99,
-   N custom λc_dollar_scope at level 99,
-   right associativity).
+Scheme tm_mut := Induction for tm Sort Prop
+with val_mut := Induction for val Sort Prop
+with non_mut := Induction for non Sort Prop.
 
-Notation "< M >" := <{ (λ 0) $ M }> (in custom λc_dollar_scope at level 0).
+Module Notations.
+  Declare Custom Entry λc_dollar_scope.
+  Notation "<{ M }>" := M (at level 1, M custom λc_dollar_scope at level 99).
+  Notation "( x )" := x (in custom λc_dollar_scope, x at level 99).
+  Notation "{ x }" := x (in custom λc_dollar_scope at level 0, x constr).
+  Notation "x" := x (in custom λc_dollar_scope at level 0, x constr at level 0).
+  Notation "'var' v" := (tm_val (val_var v)) (in custom λc_dollar_scope at level 1, left associativity).
+  Notation "0" := <{ var None }> (in custom λc_dollar_scope at level 0).
+  Notation "1" := <{ var {Some None} }> (in custom λc_dollar_scope at level 0).
+  Notation "2" := <{ var {Some (Some None)} }> (in custom λc_dollar_scope at level 0).
+  Notation "M N" := (tm_non (non_app M N)) (in custom λc_dollar_scope at level 1, left associativity).
+  Notation "'λ' M" := (tm_val (val_lam M))
+    (in custom λc_dollar_scope at level 90,
+    M custom λc_dollar_scope at level 99,
+    right associativity).
+  Notation "M '$' N" := (tm_non (non_reset M N)) (in custom λc_dollar_scope at level 80, right associativity).
+  Notation "'S₀'" := (tm_val (val_S₀)) (in custom λc_dollar_scope at level 0).
+  Notation "'S₀λ' M" := <{ {tm_val (val_S₀)} (λ M) }>
+    (in custom λc_dollar_scope at level 90,
+    M custom λc_dollar_scope at level 99,
+    right associativity).
+  Notation "'let' M 'in' N" := (tm_non (non_let M N))
+    (in custom λc_dollar_scope at level 95,
+    M custom λc_dollar_scope at level 99,
+    N custom λc_dollar_scope at level 99,
+    right associativity).
+  Notation "< M >" := <{ (λ 0) $ M }> (in custom λc_dollar_scope at level 0).
+End Notations.
+Export Notations.
+
+(* Map *)
+
+Fixpoint map {A B : Type} (f : A → B) (e : tm A) : tm B :=
+  match e with
+  | tm_val t => tm_val (map_val f t)
+  | tm_non t => tm_non (map_non f t)
+  end
+with map_val {A B : Type} (f : A → B) (e : val A) : val B :=
+  match e with
+  | val_var v => val_var (f v)
+  | val_lam e => val_lam (map (option_map f) e)
+  | val_S₀    => val_S₀
+  end
+with map_non {A B : Type} (f : A → B) (e : non A) : non B :=
+  match e with
+  | non_app e1 e2 => non_app (map f e1) (map f e2)
+  | non_let e1 e2 => non_let (map f e1) (map (option_map f) e2)
+  | non_reset e1 e2 => non_reset (map f e1) (map f e2)
+  end.
+
+Notation map_id_law_for F := (λ V e,
+  ∀ (f : V → V),
+    (∀ x, f x = x) →
+    F f e = e
+).
+
+Ltac crush := 
+  intros; cbn; f_equal; auto.
+
+Ltac crush_option := 
+  let x := fresh "x" in
+  intros [x|]; cbn; f_equal; auto.
+
+Lemma map_id_law : ∀ V e, map_id_law_for map V e.
+Proof.
+  cbn; apply (tm_mut
+    (map_id_law_for map)
+    (map_id_law_for map_val)
+    (map_id_law_for map_non)); crush;
+  (apply H + apply H0); crush_option.
+Qed.
+
+Notation map_comp_law_for F := (λ A e,
+  ∀ B C (f : A → B) (g : B → C),
+    F g (F f e) = F (g ∘ f) e
+).
+
+Lemma option_map_comp : ∀ A B C (f : A → B) (g : B → C),
+  option_map (g ∘ f) = option_map g ∘ option_map f.
+Proof.
+  intros. apply functional_extensionality. crush_option.
+Qed.
+
+Lemma map_comp_law : ∀ V e, map_comp_law_for map V e.
+Proof.
+  cbn; apply (tm_mut
+    (map_comp_law_for map)
+    (map_comp_law_for map_val)
+    (map_comp_law_for map_non)); crush;
+  rewrite option_map_comp;
+  (apply H + apply H0); crush_option.
+Qed.
+
+(* Bind *)
+
+Definition option_bind {A B} (f: A → val B) (o: ^A) : val ^B :=
+  match o with
+  | None => val_var None
+  | Some a => map_val Some (f a)
+  end.
+
+Fixpoint bind {A B : Type} (f : A → val B) (e : tm A) : tm B :=
+  match e with
+  | tm_val t => tm_val (bind_val f t)
+  | tm_non t => tm_non (bind_non f t)
+  end
+with bind_val {A B : Type} (f : A → val B) (e : val A) : val B :=
+  match e with
+  | val_var v => f v
+  | val_lam e => val_lam (bind (option_bind f) e)
+  | val_S₀    => val_S₀
+  end
+with bind_non {A B : Type} (f : A → val B) (e : non A) : non B :=
+  match e with
+  | non_app e1 e2 => non_app (bind f e1) (bind f e2)
+  | non_let e1 e2 => non_let (bind f e1) (bind (option_bind f) e2)
+  | non_reset e1 e2 => non_reset (bind f e1) (bind f e2)
+  end.
+
+Notation bind_is_map_for F Bind := (λ A e,
+  ∀ B (f : A → B), F f e = Bind (λ v, val_var (f v)) e
+).
+
+Lemma bind_is_map : ∀ A e, bind_is_map_for map bind A e.
+Proof.
+  cbn; apply (tm_mut
+    (bind_is_map_for map bind)
+    (bind_is_map_for map_val bind_val)
+    (bind_is_map_for map_non bind_non)); crush;
+    (rewrite H + rewrite H0); f_equal; apply functional_extensionality; crush_option.
+Qed.
+
+(* Notation bind_law_for Bind := (λ A e,
+  ∀ B C (f:A → val B) (g:B → val C),
+    Bind g (Bind f e) = Bind (λ a, Bind g (f a)) e
+).
+Lemma bind_law : ∀ A e, bind_law_for bind A e. *)
+
 
 (* Closed terms *)
 
@@ -67,15 +179,14 @@ Example tm_id : term := <{ λ 0 }>.
 Example tm_ω  : term := <{ λ 0 0 }>.
 Example tm_Ω  : term := <{ (λ 0 0) (λ 0 0) }>.
 
-Example tm_e1 a z b : term := <{ <a <(S₀ S₀ 1 (0 z)) b>> }>.
-Example tm_shift_id e : term := <{ S₀ 0 $ e }>.
+Example tm_e1 a z b : term := <{ <a <(S₀λ S₀λ 1 (0 z)) b>> }>.
+
+Example tm_shift_id  e : term := <{ S₀λ 0 $ e }>.
 
 (* Contexts *)
 
 Section Contexts.
-
   Context {V : Type}.
-
   Inductive J :=
   | J_app_l : tm V → J   (* [] M *)
   | J_app_r : val V → J  (* V [] *)
@@ -90,7 +201,6 @@ Section Contexts.
   | E_K : K → E → E
   | E_V : val V → E → E
   .
-
 End Contexts.
 Arguments J V : clear implicits.
 Arguments K V : clear implicits.
